theory/Sound_Semantics.thy
@@ -1505,10 +1505,6 @@ proof -
   show " {|\<omega>|} \<subseteq> \<V> x" using trace_pool_always_not_static_bound_sound by blast
 qed
 
-
-
-(*
-
 inductive static_reachable :: "exp \<Rightarrow> exp \<Rightarrow> bool"  where
   Refl : "
     static_reachable e e
@@ -2099,6 +2095,5 @@ proof -
     by fastforce
 qed
 
-*)
 
 end
